WIP: Running example

io/RunningExample.fst
@@ -5,6 +5,8 @@ open FStar.List.Tot.Base
 
 open Compiler.Model
 
+
+(** ** Temporary redefining types *)
 type access_policy = (history:trace) -> (isTrusted:bool) -> (cmd:io_cmds) -> (io_sig.args cmd) -> Type0
 
 (** TODO: show that the type of access_policy is enough to enforce any monitorable property
@@ -35,7 +37,7 @@ let pi_as_hist (#a:Type) (pi:access_policy) : hist a =
 effect IIOpi (a:Type) (fl:FStar.Ghost.erased tflag) (pi : access_policy) = 
   IIOwp a fl (pi_as_hist #a pi)
 
-
+(** ** Type of source handler **)
 assume val valid_http_response : string -> bool
 assume val valid_http_request : string -> bool
 
@@ -49,8 +51,8 @@ val handler_only_openfiles_reads_client_acc : trace -> list file_descr -> bool
 let rec handler_only_openfiles_reads_client_acc lt open_descrs =
   match lt with
   | [] -> true
-  | EOpenfile true  _ _ :: tl -> handler_only_openfiles_reads_client_acc tl open_descrs
-  | ERead true  _ _ :: tl -> handler_only_openfiles_reads_client_acc tl open_descrs
+  | EOpenfile true  _ _ :: tl -> false
+  | ERead true  _ _ :: tl -> false
   | EWrite true _ _ :: tl -> handler_only_openfiles_reads_client_acc tl open_descrs
   | EClose true  _ _ :: tl -> handler_only_openfiles_reads_client_acc tl open_descrs
   | EOpenfile false fnm res :: tl -> 
@@ -71,6 +73,112 @@ val handler_only_openfiles_reads_client : trace -> bool
 let handler_only_openfiles_reads_client lt =
   handler_only_openfiles_reads_client_acc lt []
 
+val wrote_at_least_once_to : file_descr -> trace -> bool
+let rec wrote_at_least_once_to client lt =
+  match lt with
+  | [] -> false
+  | EWrite true arg _::tl -> let (fd, msg):file_descr*string = arg in
+                         client = fd
+  | _ :: tl -> wrote_at_least_once_to client tl 
+
+type request_handler =
+  (client:file_descr) ->
+  (req:string) ->
+  (send:(msg:string -> IIO (resexn unit) IOActions (requires (fun h -> valid_http_response msg /\
+                                                                      did_not_respond h))
+                                                   (ensures (fun _ _ lt -> exists r. lt == [EWrite true (client,msg) r] /\
+                                                                         wrote_at_least_once_to client lt)))) ->
+  IIO (resexn unit) IOActions (requires (fun h -> valid_http_request req /\ did_not_respond h))
+                              (ensures (fun h _ lt -> handler_only_openfiles_reads_client lt /\
+                                                    wrote_at_least_once_to client lt))
+
+(** ** E.g. of source handler **)
+assume val req_res : req:string{valid_http_request req} -> res:string{valid_http_response res}
+
+val source_handler : request_handler
+let source_handler client req send =
+  let res = req_res req in
+  let _ = send res in 
+  Inl ()
+
+type acts (fl:erased tflag) (pi:access_policy) (isTrusted:bool) =
+  (cmd : io_cmds) ->
+  (arg : io_sig.args cmd) ->
+  IIO (io_resm cmd arg) fl
+    (requires (fun _ -> True))
+    (ensures (fun h r lt ->
+      enforced_locally pi h lt /\
+      (match r with
+       | Inr Contract_failure -> lt == []
+       | r' -> lt == [convert_call_to_event isTrusted cmd arg r'])))
+
+
+(** ** E.g. of target handler **)
+type tgt_handler =
+  (fl:erased tflag) ->
+  (pi:erased access_policy) ->
+  (io_acts:acts fl pi false) ->
+  (client:file_descr) ->
+  (req:string) ->
+  (send:(msg:string -> IIOpi (resexn unit) fl pi)) ->
+  IIOpi (resexn unit) fl pi
+
+val target_handler1 : tgt_handler
+let target_handler1 fl pi io_acts client req send =
+  let _ = send req in 
+  Inl ()
+
+val target_handler2 : tgt_handler
+let target_handler2 fl pi io_acts client req send =
+  let _ = io_acts Openfile "/etc/passwd" in
+  let _ = send req in 
+  Inl ()
+
+(** ** Source webserver **)
+val every_request_gets_a_response_acc : trace -> list file_descr -> Type0
+let rec every_request_gets_a_response_acc lt read_descrs =
+  match lt with
+  | [] -> read_descrs == []
+  | ERead true fd (Inl _)::tl -> every_request_gets_a_response_acc tl (fd::read_descrs)
+  | EWrite true (fd,_) _::tl -> every_request_gets_a_response_acc tl (filter (fun fd' -> fd <> fd') read_descrs)
+  | _::tl -> every_request_gets_a_response_acc tl read_descrs
+
+val every_request_gets_a_response : trace -> Type0
+let every_request_gets_a_response lt =
+  every_request_gets_a_response_acc lt []
+
+assume val get_req : file_descr -> option (req:string{valid_http_request req})
+assume val sendError : int -> fd:file_descr -> IIO unit IOActions
+ (fun _ -> True) (fun _ _ lt -> exists (msg:string) r. lt == [EWrite true (fd, msg) r])
+
+open FStar.Tactics
+(* This may take a bit of effort to prove. *)
+let webserver (handler:request_handler) :
+  IIO (resexn unit) IOActions
+    (requires (fun h -> True))
+    (ensures (fun _ _ lt -> 
+      every_request_gets_a_response lt))
+    by (
+      explode ();
+      bump_nth 49; 
+      l_to_r [`FStar.List.Tot.Properties.append_nil_l];
+      let l = instantiate (nth_binder 3) (fresh_uvar None) in
+      let l = instantiate l (nth_binder (-3)) in
+      mapply l;
+      binder_retype (nth_binder (-3));
+        l_to_r [`FStar.List.Tot.Properties.append_nil_l];
+      trefl ();
+      tadmit ();
+      dump "H") =
+  let client = static_cmd true Openfile "test.txt" in
+  match client with | Inr err -> Inr err | Inl client -> begin
+    match get_req client with
+    | Some req -> handler client req (fun res -> static_cmd true Write (client,res))
+    | None -> sendError 400 client;
+    static_cmd true Close client
+  end
+
+(** ** Instante source interface with the example **)
 let rec is_opened_by_untrusted (h:trace) (fd:file_descr) : bool =
   match h with
   | [] -> false
@@ -98,89 +206,4 @@ let rec lemma1 (lt h:trace) : Lemma (requires (enforced_locally pi h lt)) (ensur
   | e::tl -> admit ()//  lemma1 tl (e::h)
 
 
-val wrote_at_least_once_to : file_descr -> trace -> bool
-let rec wrote_at_least_once_to client lt =
-  match lt with
-  | [] -> false
-  | EWrite true arg _::tl -> let (fd, msg):file_descr*string = arg in
-                         client = fd
-  | _ :: tl -> wrote_at_least_once_to client tl 
-
-type request_handler =
-  (client:file_descr) ->
-  (req:string) ->
-  (send:(msg:string -> IIO (resexn unit) IOActions (requires (fun h -> valid_http_response msg /\
-                                                                      did_not_respond h))
-                                                   (ensures (fun _ _ lt -> exists r. lt == [EWrite true (client,msg) r] /\
-                                                                         wrote_at_least_once_to client lt)))) ->
-  IIO (resexn unit) IOActions (requires (fun h -> valid_http_request req /\ did_not_respond h))
-                              (ensures (fun h _ lt -> enforced_locally pi h lt /\
-                                                    wrote_at_least_once_to client lt))
-
-assume val req_res : req:string{valid_http_request req} -> res:string{valid_http_response res}
-
-val source_handler : request_handler
-let source_handler client req send =
-  let res = req_res req in
-  let _ = send res in 
-  Inl ()
-
-val every_request_gets_a_response_acc : trace -> list file_descr -> Type0
-let rec every_request_gets_a_response_acc lt read_descrs =
-  match lt with
-  | [] -> read_descrs == []
-  | ERead true fd (Inl _)::tl -> every_request_gets_a_response_acc tl (fd::read_descrs)
-  | EWrite true (fd,_) _::tl -> every_request_gets_a_response_acc tl (filter (fun fd' -> fd <> fd') read_descrs)
-  | _::tl -> every_request_gets_a_response_acc tl read_descrs
-
-val every_request_gets_a_response : trace -> Type0
-let every_request_gets_a_response lt =
-  every_request_gets_a_response_acc lt []
-
-assume val get_req : file_descr -> option (req:string{valid_http_request req})
-assume val sendError : int -> fd:file_descr -> IIO unit IOActions
- (fun _ -> True) (fun _ _ lt -> exists (msg:string) r. lt == [EWrite true (fd, msg) r])
-
-open FStar.Tactics
-
-(* This may take a bit of effort to prove. *)
-
-let webserver (handler:request_handler) :
-  IIO (resexn unit) IOActions
-    (requires (fun h -> True))
-    (ensures (fun _ _ lt -> 
-      every_request_gets_a_response lt))
-    by (
-      explode ();
-      bump_nth 49; 
-      l_to_r [`FStar.List.Tot.Properties.append_nil_l];
-      let l = instantiate (nth_binder 3) (fresh_uvar None) in
-      let l = instantiate l (nth_binder (-3)) in
-      mapply l;
-      binder_retype (nth_binder (-3));
-        l_to_r [`FStar.List.Tot.Properties.append_nil_l];
-      trefl ();
-      tadmit ();
-      dump "H") =
-  let client = static_cmd true Openfile "test.txt" in
-  match client with | Inr err -> Inr err | Inl client -> begin
-    match get_req client with
-    | Some req -> handler client req (fun res -> static_cmd true Write (client,res))
-    | None -> sendError 400 client;
-    static_cmd true Close client
-  end
-
-
-type tgt_handler =
-  (fl:erased tflag) ->
-  (pi:erased access_policy) ->
-  (io_acts:acts fl pi false) ->
-  (client:file_descr) ->
-  (req:string) ->
-  (send:(msg:string -> IIOpi (resexn unit) fl pi)) ->
-  IIOpi (resexn unit) fl pi
-
-val target_handler : tgt_handler
-let target_handler fl pi io_acts client req send =
-  let _ = send req in 
-  Inl ()
+(** ** Tests: compile web-server, back-translate handler, linking **)
